Fix empty star (#162)
* Change star compilation

* Move pushRegex_get_lt to regex

* Basic fix for correctness

* Adapt ProofData for new compilation

* Adapt Correctness.NFA.Compile for new compilation

* Adapt most of the proofs

* Fix proof of PathOfCaptures

* Add comment

correctness/RegexCorrectness/NFA/Semantics/ProofData/Loop.lean
@@ -10,23 +10,24 @@ namespace Regex.NFA.Compile.ProofData.Star
 variable [Star]
 
 /--
-Consider `nfa' := nfa.pushRegex next e`. When there is a path in `nfa'` from `nfa'.start` to `next`,
-it must have looped `nfaExpr` before `n` times, followed by the last step from `nfa'.start` to `next`.
+Consider `nfa' := nfa.pushRegex next (.star greedy e)`. When there is a path in `nfa'` from `nfaExpr.start` to `next`,
+it must have looped `nfaExpr` before `n` times, followed by the last step from `nfa.size` to `next`.
 
 A `Loop` term corresponds to such a loop. The `last` variant corresponds to the last step,
 and the `loop` variant extracts the first iteration and the remaining loop.
 -/
 public inductive Loop {s : String} : Pos s → Pos s → List (Nat × Pos s) → Prop where
-  | last {pos} (step : nfa'.Step nfa.size nfa'.start pos next pos .none) : Loop pos pos []
+  | last {pos} (step : nfa'.Step nfa.size nfa.size pos next pos .none) : Loop pos pos []
   | loop {pos pos' pos'' update₁ update₂}
     (path : nfa'.Path nfaPlaceholder.size nfaExpr.start pos nfaPlaceholder.start pos' update₁)
-    (loop : Loop pos' pos'' update₂) : Loop pos pos'' (update₁ ++ update₂)
+    (loop : Loop pos' pos'' update₂) :
+    Loop pos pos'' (update₁ ++ update₂)
 
 theorem Loop.introAux {s : String} {pos pos' : Pos s} {i j update}
-  (lt : i < nfa'.size) (wf : nfa.WellFormed) (next_lt : next < nfa.size) (eqj : j = next)
+  (lt : i < nfaExpr.size) (wf : nfa.WellFormed) (next_lt : next < nfa.size) (eqj : j = next)
   (path : nfa'.Path nfa.size i pos j pos' update) :
-  if i = nfa'.start then
-    (nfa'.Step nfa.size nfa'.start pos next pos' .none ∧ pos' = pos ∧ update = []) ∨
+  if i = nfa.size then
+    (nfa'.Step nfa.size nfa.size pos next pos' .none ∧ pos' = pos ∧ update = []) ∨
     (∃ posm update₁ update₂,
       nfa'.Path nfaPlaceholder.size nfaExpr.start pos nfaPlaceholder.start posm update₁ ∧
       Loop posm pos' update₂ ∧
@@ -38,96 +39,75 @@ theorem Loop.introAux {s : String} {pos pos' : Pos s} {i j update}
       update = update₁ ++ update₂ := by
   induction path with
   | @last i pos j pos' update step =>
-    split
+    have get := get i (by grind)
+    split_ifs at get
+    next => grind
     next eqi =>
-      subst eqi eqj
-      simp only [step_start_iff, or_true, true_and] at step
-      simp only [step, List.ofOption_none, and_self, and_true, List.nil_eq, List.append_eq_nil_iff,
-        exists_and_left, ↓existsAndEq, exists_eq_right_right]
-
-      have wf' := wf' wf next_lt
-      have : nfa'[nfa'.start]'wf'.start_lt = splitNode := by
-        simp [start_eq, get_start]
-      simp only [splitNode] at this
-
-      split at this
-      . exact .inl (.splitRight (Nat.le_of_eq start_eq.symm) wf'.start_lt this)
-      . exact .inl (.splitLeft (Nat.le_of_eq start_eq.symm) wf'.start_lt this)
-    next nei =>
-      have : nfa.size ≤ i := step.ge
-      have : i ≠ nfa.size := start_eq ▸ nei
-      have gt : i > nfa.size := by grind
-
-      have step : nfa'.Step (nfa.size + 1) i pos j pos' update :=
-        step.liftBound' gt
-      have step : nfa'.Step nfaPlaceholder.size i pos j pos' update := by
-        simp [nfaPlaceholder, step]
-      have step : nfaExpr.Step nfaPlaceholder.size i pos j pos' update :=
-        step.cast (get_ne_start i step.lt (Nat.ne_of_gt gt))
-
-      have := step.eq_or_ge_of_pushRegex
-      simp only [eqj, nfaPlaceholder, pushNode_start_eq, pushNode_size] at this
-      grind
+      simp only [eqi, ↓reduceIte]
+      cases step
+      case splitLeft k ge lt' eq =>
+        simp only [eqi, eqj] at eq
+        exact .inl ⟨.splitLeft (Nat.le_refl _) size_lt eq, rfl, rfl⟩
+      case splitRight k ge lt' eq =>
+        simp only [eqi, eqj] at eq
+        exact .inl ⟨.splitRight (Nat.le_refl _) size_lt eq, rfl, rfl⟩
+      all_goals grind
+    next ne =>
+      have stepExpr : nfaExpr.Step nfa.size i pos j pos' update := step.cast get
+      have stepExpr' : nfaExpr.Step nfaPlaceholder.size i pos j pos' update := stepExpr.liftBound' (by grind)
+      grind [stepExpr'.eq_or_ge_of_pushRegex]
   | @more i pos j pos' k pos'' update₁ update₂ step rest ih =>
-    have ih' := ih rest.lt eqj
-    split
+    have get := get i (by grind)
+    split_ifs at get
+    next => grind
     next eqi =>
-      subst eqi eqj
-      have : j ≠ next := by
-        have : nfa.size ≤ j := rest.ge
-        omega
-      simp [step_start_iff, this] at step
-
-      have ne : nfaExpr.start ≠ nfa'.start := by
-        have : nfaPlaceholder.size ≤ nfaExpr.start := ge_pushRegex_start rfl
-        simp [nfaPlaceholder] at this
-        simp [start_eq]
-        omega
-      simp [step, ne] at ih'
-      simp [step]
-      exact .inr ih'
+      simp only [eqi, ↓reduceIte]
+      if hg : greedy then
+        cases _x : step
+        case splitLeft l ge lt' eq =>
+          simp only [eq, split, hg, ↓reduceIte, Node.split.injEq] at get
+          have ih := ih (by grind) eqj
+          simp only [show j ≠ nfa.size by grind, ↓reduceIte] at ih
+          obtain ⟨posm, update₃, update₄, path', loop', equ⟩ := ih
+          exact .inr ⟨posm, update₃, update₄, get.1 ▸ path', loop', by simp [equ]⟩
+        all_goals grind
+      else
+        cases step
+        case splitRight l ge lt' eq =>
+          simp only [eq, split, hg, Bool.false_eq_true, ↓reduceIte, Node.split.injEq] at get
+          have ih := ih (by grind) eqj
+          simp only [show j ≠ nfa.size by grind, ↓reduceIte] at ih
+          obtain ⟨posm, update₃, update₄, path', loop', equ⟩ := ih
+          exact .inr ⟨posm, update₃, update₄, get.2 ▸ path', loop', by simp [equ]⟩
+        all_goals grind
     next nei =>
-      have gt : i > nfa.size := by
-        simp [start_eq] at nei
-        have := step.ge
-        omega
-      split at ih'
+      simp only [nei, ↓reduceIte]
+      have step : nfa'.Step nfaPlaceholder.size i pos j pos' update₁ := step.liftBound' (by grind)
+      have stepExpr := step.cast get
+      have ih := ih (stepExpr.lt_right (wfExpr wf)) eqj
+      split at ih
       next eqj =>
-        match ih' with
+        match ih with
         | .inl ⟨step', hpos, hupdate⟩ =>
-          simp [hpos, hupdate, eqj] at *
-          refine ⟨pos', List.ofOption update₁, ?_, [], .last step', by simp⟩
-          simp [nfaPlaceholder]
-
-          have path := Path.last (step.liftBound' gt)
-          exact start_eq ▸ path
-        | .inr ⟨itm, update₃, update₄, path', loop', equ⟩ =>
-          have loop'' := Loop.loop path' loop'
-          refine ⟨pos', List.ofOption update₁, update₃ ++ update₄, ?_, loop'', by simp [equ]⟩
-          simp [nfaPlaceholder]
-
-          have step : nfa'.Step nfa.size i pos nfa.size pos' update₁ :=
-            have : j = nfa.size := eqj ▸ start_eq
-            this ▸ step
-          exact (.last (step.liftBound' gt))
+          subst pos'' update₂ j
+          exact ⟨pos', List.ofOption update₁, [], .last (by grind), .last step', by simp⟩
+        | .inr ⟨posm, update₃, update₄, path', loop', equ⟩ =>
+          have := Loop.loop path' loop'
+          exact ⟨pos', List.ofOption update₁, update₃ ++ update₄, .last (by grind), .loop path' loop', by simp [equ]⟩
       next nej =>
-        have ⟨itm, update₃, update₄, path', loop', equ⟩ := ih'
-        have step : nfa'.Step nfaPlaceholder.size i pos j pos' update₁ := by
-          simp [nfaPlaceholder]
-          exact step.liftBound' gt
-        exact ⟨itm, update₁ ::ₒ update₃, update₄, .more step path', loop', by simp [equ]⟩
+        obtain ⟨posm, update₃, update₄, path', loop', equ⟩ := ih
+        have := Path.more step path'
+        exact ⟨posm, update₁ ::ₒ update₃, update₄, .more step path', loop', by simp [equ]⟩
 
 public theorem Loop.intro {s : String} {pos pos' : Pos s} {update}
   (wf : nfa.WellFormed) (next_lt : next < nfa.size)
-  (path : nfa'.Path nfa.size nfa'.start pos next pos' update) :
+  (path : nfa'.Path nfa.size nfaExpr.start pos next pos' update) :
   Loop pos pos' update := by
-  have wf' := wf' wf next_lt
-  have loop := introAux wf'.start_lt wf next_lt rfl path
-  simp at loop
-  match loop with
-  | .inl ⟨step, hpos, hupdate⟩ =>
-    simp [hpos, hupdate] at *
-    exact .last step
-  | .inr ⟨pos'', update₁, path, update₂, loop, equ⟩ => exact equ ▸ Loop.loop path loop
+  have loop := introAux (by grind) wf next_lt rfl path
+  split at loop
+  next => grind
+  next =>
+    obtain ⟨posm, update₁, update₂, path', loop', equ⟩ := loop
+    exact equ ▸ Loop.loop path' loop'
 
 end Regex.NFA.Compile.ProofData.Star
