correctness/RegexCorrectness/NFA/Semantics/Equivalence/PathOfCaptures.lean
@@ -23,8 +23,8 @@ theorem path_of_captures.group {tag} (eq : nfa.pushRegex next (.group tag e) = r
   let pd := Group.intro eq
   simp [eq_result eq]
 
-  have wf_close := wf_close wf next_lt
-  have ⟨update, eqv, path⟩ := ih (result := nfaExpr) rfl wf_close wf_close.start_lt
+  have wfClose := wfClose wf next_lt
+  have ⟨update, eqv, path⟩ := ih (result := nfaExpr) rfl wfClose wfClose.start_lt
   exists (2 * tag, pos) :: update ++ [(2 * tag + 1, pos')], .group eqv
 
   have stepOpen : nfa'.Step nfa.size nfa'.start pos nfaExpr.start pos (.some (2 * tag, pos)) := by
@@ -119,22 +119,29 @@ theorem path_of_captures.starConcat {pos'' greedy e groups₁ groups₂} (eq : n
   let pd := Star.intro eq
   simp [pd.eq_result eq]
 
-  have wf_placeholder := wf_placeholder wf
-  have ⟨update₁, eqv₁, path₁⟩ := ih₁ (result := nfaExpr) rfl wf_placeholder wf_placeholder.start_lt
+  have wfPlaceholder := wfPlaceholder wf
+  have ⟨update₁, eqv₁, path₁⟩ := ih₁ (result := nfaExpr) (by grind only [= nfaPlaceholder,
+    = Star.intro, = nfaExpr, = pushNode_start]) wfPlaceholder wfPlaceholder.start_lt
   have ⟨update₂, eqv₂, path₂⟩ := ih₂ (result := nfa') rfl wf next_lt
   exists update₁ ++ update₂, .concat eqv₁ eqv₂
 
-  have start_eq_placeholder : nfaPlaceholder.start = nfa'.start := by
-    simp [nfaPlaceholder, start_eq]
-  have path₁ : nfa'.Path nfa.size nfaExpr.start pos nfa'.start pos' update₁ :=
-    start_eq_placeholder ▸ (castFromExpr path₁).liftBound (by simp [nfaPlaceholder]; exact Nat.le_succ _)
-  have step : nfa'.Step nfa.size nfa'.start pos nfaExpr.start pos .none :=
-    if h : pd.greedy then
-      .splitLeft (j₂ := next) (by simp [start_eq]; exact Nat.le_refl _) (wf' wf next_lt).start_lt (by simp [start_eq, get_start, splitNode, h]; rfl)
-    else
-      .splitRight (j₁ := next) (by simp [start_eq]; exact Nat.le_refl _) (wf' wf next_lt).start_lt (by simp [start_eq, get_start, splitNode, h]; rfl)
+  have wf' : nfa'.WellFormed := pushRegex_wf wf next_lt
 
-  exact (Path.more step path₁).trans path₂
+  have path₁ : nfa'.Path nfa.size nfaExpr.start pos nfaPlaceholder.start pos' update₁ :=
+    (castFromExpr path₁).liftBound (by grind only [nfaPlaceholder, Star.intro, = pushNode_size])
+  have step : nfa'.Step nfa.size nfa'.start pos nfaExpr.start pos .none :=
+    step_start_iff.mpr ⟨.inl rfl, rfl, rfl⟩
+  have path₁ : nfa'.Path nfa.size nfa'.start pos nfaPlaceholder.start pos' update₁ :=
+    .more step path₁
+
+  have path₂ : nfa'.Path nfa.size nfaPlaceholder.start pos' next pos'' update₂ := by
+    apply path₂.castHead
+    . simp [pd.get_placeholder_start, pd.get_start]
+    . grind only [nfaPlaceholder, Star.intro, = start.eq_1, = pushNode_start]
+    . exact wf'.start_lt
+    . exact path₁.lt_right wf'
+
+  exact path₁.trans path₂
 
 public theorem path_of_captures (eq : nfa.pushRegex next e = result)
   (wf : nfa.WellFormed) (next_lt : next < nfa.size)
