correctness/RegexCorrectness/NFA/Semantics/ProofData/Cast.lean
@@ -18,15 +18,15 @@ theorem castFromExpr (path : nfaExpr.Path nfaClose.size nfaExpr.start pos nfaClo
   nfa'.Path nfaClose.size nfaExpr.start pos nfaClose.start pos' update := by
   apply path.cast
   intro i _ lt
-  exact ⟨Nat.lt_trans lt size_lt_expr', (get_lt_expr lt).symm⟩
+  exact ⟨Nat.lt_trans lt size_lt_expr', by grind⟩
 
 theorem castToExpr {lb j} (wf : nfa.WellFormed) (next_lt : next < nfa.size)
   (path : nfa'.Path lb nfaExpr.start pos j pos' update) :
   nfaExpr.Path lb nfaExpr.start pos j pos' update := by
-  have wf_expr := wf_expr wf next_lt
-  apply path.cast' wf_expr.start_lt (Nat.le_of_lt size_lt_expr') wf_expr
+  have wfExpr := wfExpr wf next_lt
+  apply path.cast' wfExpr.start_lt (Nat.le_of_lt size_lt_expr') wfExpr
   intro i _ lt
-  exact get_lt_expr lt
+  grind
 
 end Group
 
@@ -38,13 +38,13 @@ theorem castFrom₁ (path : nfa₁.Path nfa.size nfa₁.start pos next pos' upda
   nfa'.Path nfa.size nfa₁.start pos next pos' update := by
   apply path.cast
   intro i _ lt
-  exact ⟨Nat.lt_trans lt size_lt₁, (get_lt₁ lt).symm⟩
+  exact ⟨Nat.lt_trans lt size_lt₁, by grind⟩
 
 theorem castFrom₂ (path : nfa₂.Path nfa.size nfa₂.start pos next pos' update) :
   nfa'.Path nfa.size nfa₂.start pos next pos' update := by
   apply path.cast
   intro i _ lt
-  exact ⟨Nat.lt_trans lt size_lt₂, (get_lt₂ lt).symm⟩
+  exact ⟨Nat.lt_trans lt size_lt₂, by grind⟩
 
 theorem castTo₁ (wf : nfa.WellFormed) (next_lt : next < nfa.size)
   (path : nfa'.Path nfa.size nfa₁.start pos next pos' update) :
@@ -52,7 +52,7 @@ theorem castTo₁ (wf : nfa.WellFormed) (next_lt : next < nfa.size)
   have wf₁ := wf₁ wf next_lt
   apply path.cast' wf₁.start_lt (Nat.le_of_lt size_lt₁) wf₁
   intro i _ lt
-  exact get_lt₁ lt
+  grind
 
 theorem castTo₂ {lb} (wf : nfa.WellFormed) (next_lt : next < nfa.size)
   (path : nfa'.Path lb nfa₂.start pos next pos' update) :
@@ -60,7 +60,7 @@ theorem castTo₂ {lb} (wf : nfa.WellFormed) (next_lt : next < nfa.size)
   have wf₂ := wf₂ wf next_lt
   apply path.cast' wf₂.start_lt (Nat.le_of_lt size_lt₂) wf₂
   intro i _ lt
-  exact get_lt₂ lt
+  grind
 
 end Alternate
 
@@ -72,7 +72,7 @@ theorem castFrom₂ (path : nfa₂.Path nfa.size nfa₂.start pos next pos' upda
   nfa'.Path nfa.size nfa₂.start pos next pos' update := by
   apply path.cast
   intro i _ lt
-  exact ⟨Nat.lt_trans lt size₂_lt, (get_lt₂ lt).symm⟩
+  exact ⟨Nat.lt_trans lt size₂_lt, by grind⟩
 
 theorem castTo₂ (wf : nfa.WellFormed) (next_lt : next < nfa.size)
   (path : nfa'.Path nfa.size nfa₂.start pos next pos' update) :
@@ -80,7 +80,7 @@ theorem castTo₂ (wf : nfa.WellFormed) (next_lt : next < nfa.size)
   have wf₂ := wf₂ wf next_lt
   apply path.cast' wf₂.start_lt (Nat.le_of_lt size₂_lt) wf₂
   intro i _ lt
-  exact get_lt₂ lt
+  grind
 
 end Concat
 
@@ -93,16 +93,16 @@ theorem castFromExpr (path : nfaExpr.Path nfaPlaceholder.size nfaExpr.start pos 
   apply path.cast
   intro i ge lt
   simp [nfaPlaceholder] at ge
-  exact ⟨size_eq_expr' ▸ lt, (get_ne_start i (size_eq_expr' ▸ lt) (Nat.ne_of_gt ge)).symm⟩
+  exact ⟨by grind, by grind⟩
 
 theorem castToExpr (wf : nfa.WellFormed)
   (path : nfa'.Path nfaPlaceholder.size nfaExpr.start pos nfaPlaceholder.start pos' update) :
   nfaExpr.Path nfaPlaceholder.size nfaExpr.start pos nfaPlaceholder.start pos' update := by
-  have wf_expr := wf_expr wf
-  apply path.cast' wf_expr.start_lt (Nat.le_of_eq size_eq_expr'.symm) wf_expr
+  have wfExpr := wfExpr wf
+  apply path.cast' wfExpr.start_lt (by grind) wfExpr
   intro i ge lt
   simp [nfaPlaceholder] at ge
-  exact (get_ne_start i (size_eq_expr' ▸ lt) (Nat.ne_of_gt ge))
+  grind
 
 end Star
 
