correctness/RegexCorrectness/VM/Search/Compile.lean
@@ -19,10 +19,10 @@ theorem captures_of_some_compile {s e pos₀ matched'} (h : captureNext (History
     e.Captures pos pos' groups ∧
     EquivUpdate groups (matched'.get isSome') := by
   have ⟨state, pos', hn, path⟩ := path_done_of_matched h isSome'
-  have eq_zero := (NFA.done_iff_zero_compile rfl state).mp hn
+  have eq_zero := (NFA.done_iff_zero_compile state state.isLt).mp hn
   have : state.val ≠ (NFA.compile e).start := by
     simp [eq_zero]
-    exact Nat.ne_of_lt (NFA.lt_zero_start_compile rfl)
+    exact Nat.ne_of_lt NFA.lt_zero_start_compile
   have ⟨pos, le, path⟩ := path.nfaPath_of_ne this
   simp [eq_zero] at path
   have ⟨groups, eqv, c⟩ := NFA.captures_of_path_compile rfl (path.compile_liftBound rfl)
@@ -32,11 +32,11 @@ theorem not_captures_of_none_compile {s e pos} (h : captureNext (HistoryStrategy
   (pos' pos'' : Pos s) (groups : CaptureGroups s) (le : pos ≤ pos') :
   ¬e.Captures pos' pos'' groups := by
   intro c
-  let zero : Fin (NFA.compile e).size := ⟨0, NFA.lt_zero_size_compile rfl⟩
+  let zero : Fin (NFA.compile e).size := ⟨0, NFA.lt_zero_size_compile⟩
   have ⟨update, _, path⟩ := NFA.path_of_captures_compile rfl c
   have path := NFA.VMPath.of_nfaPath NFA.compile_wf le (path.liftBound (by decide))
   have ne := ne_done_of_path_of_none h pos'' zero update path
-  exact ne ((NFA.done_iff_zero_compile rfl zero).mpr rfl)
+  exact ne ((NFA.done_iff_zero_compile zero (by grind)).mpr (by simp [zero]))
 
 end captureNext
 
