regex/Regex/NFA/Compile/Lemmas.lean
@@ -3,37 +3,58 @@ module
 public import Regex.NFA.Compile.Basic
 import all Regex.NFA.Compile.Basic
 
+public section
+
 namespace Regex.NFA
 
-public theorem pushRegex_size_lt {nfa : NFA} {next e} :
+@[grind! .]
+theorem pushRegex_size_lt {nfa : NFA} {next e} :
   nfa.size < (nfa.pushRegex next e).size := by
-  induction e generalizing nfa next with
-  | empty => simp [pushRegex]
-  | epsilon => simp [pushRegex]
-  | anchor a => simp [pushRegex]
-  | char => simp [pushRegex]
-  | classes => simp [pushRegex]
-  | group tag e ih =>
-    simp [pushRegex]
+  fun_induction pushRegex
+  -- star
+  case case9 nfa next greedy e patchAt placeholder compiled split quest patched ih =>
     calc nfa.size
-      _ < (nfa.pushNode (.save (2 * tag + 1) next)).size := by simp
-      _ < ((nfa.pushNode (.save (2 * tag + 1) next)).pushRegex nfa.size e).size := ih
-      _ < _ := by omega
-  | alternate e₁ e₂ ih₁ ih₂ =>
-    simp [pushRegex]
-    calc nfa.size
-      _ < (nfa.pushRegex next e₁).size := ih₁
-      _ < ((nfa.pushRegex next e₁).pushRegex next e₂).size := ih₂
-      _ < _ := by omega
-  | concat e₁ e₂ ih₁ ih₂ =>
-    simp [pushRegex]
-    calc nfa.size
-      _ < (nfa.pushRegex next e₂).size := ih₂
-      _ < _ := ih₁
-  | star greedy e ih =>
-    simp [pushRegex, size]
-    calc nfa.size
-      _ < (nfa.pushNode .fail).size := by simp
-      _ < ((nfa.pushNode .fail).pushRegex nfa.size e).size := ih
+      _ < placeholder.size := by grind
+      _ < compiled.size := ih
+      _ < quest.size := by grind
+      _ = _ := by grind
+  all_goals grind
+
+@[grind! .]
+theorem pushRegex_wf {nfa : NFA} {next e} (wf : nfa.WellFormed) (next_lt : next < nfa.size) :
+  (nfa.pushRegex next e).WellFormed := by
+  fun_induction pushRegex
+  -- star
+  case case9 nfa next greedy e patchAt placeholder compiled split quest patched ih =>
+    have lt₁ : compiled.start < quest.size := by grind
+    have lt₂ : next < quest.size := by grind
+    have wfCompiled : compiled.WellFormed := ih (pushNode_wf wf (by grind)) (by grind)
+    have wfQuest : quest.WellFormed := pushNode_wf wfCompiled (by grind)
+    refine WellFormed.iff.mpr ⟨by grind [wfQuest.size_lt], ?_⟩
+    intro i h
+    if eq : i = patchAt then
+      grind
+    else
+      grind [wfQuest.inBounds i (by grind)]
+  all_goals grind
+
+theorem compile_wf {e} : (compile e).WellFormed :=
+  pushRegex_wf done_WellFormed done_WellFormed.size_lt
+
+@[grind =]
+theorem pushRegex_get_lt {nfa next e} (i : Nat) (h : i < nfa.size) :
+  (pushRegex nfa next e)[i]'(Nat.lt_trans h pushRegex_size_lt) = nfa[i] := by
+  fun_induction pushRegex nfa next e
+  -- star
+  case case9 nfa next greedy e patchAt placeholder compiled split quest patched ih =>
+    have eq : pushRegex nfa next (.star greedy e) = patched := rfl
+    simp only [eq]
+    conv =>
+      lhs
+      rw [get_eq_nodes_get, Array.getElem_setIfInBounds_ne (by grind) (by grind)]
+      rw [←get_eq_nodes_get, pushNode_get_lt i (by grind), ih (by grind), pushNode_get_lt i (by grind)]
+  all_goals grind
 
 end Regex.NFA
+
+end
